src/ADTRefinement/GeneralBuildADTRefinements.v
@@ -19,79 +19,79 @@ Section BuildADTRefinements.
   Require Import Coq.Strings.String.
   Local Hint Resolve string_dec.
 
-  Lemma refineADT_BuildADT_ReplaceConstructor
-        (Rep : Type)
-        (AbsR : Rep -> Rep -> Prop)
-        {n n'}
-        (consSigs : Vector.t consSig n)
-        (methSigs : Vector.t methSig n')
-        (consDefs : ilist (B := @consDef Rep) consSigs)
-        (methDefs : ilist (B := @methDef Rep) methSigs)
-        (idx : @Fin.t n)
-        (newDef : consDef (Vector.nth consSigs idx))
-  :
-    (forall consIdx,
-       refineConstructor AbsR (getConsDef consDefs consIdx) (getConsDef consDefs consIdx))
-    -> (forall methIdx,
-          refineMethod AbsR (getMethDef methDefs methIdx) (getMethDef methDefs methIdx))
-    -> refineConstructor AbsR
-                         (consBody (ith consDefs idx ))
-                         (consBody newDef)
-    -> refineADT
-         (BuildADT consDefs methDefs)
-         (ADTReplaceConsDef consDefs methDefs idx newDef).
-  Proof.
-    intros; eapply refineADT_BuildADT_Rep with (AbsR := AbsR); eauto.
-    intros; unfold getConsDef.
-    unfold replaceConsDef.
-    destruct (fin_eq_dec consIdx idx); subst.
-    rewrite ith_replace_Index_eq; eauto.
-    rewrite ith_replace_Index_neq; eauto.
-  Qed.
+  (* Lemma refineADT_BuildADT_ReplaceConstructor *)
+  (*       (Rep : Type) *)
+  (*       (AbsR : Rep -> Rep -> Prop) *)
+  (*       {n n'} *)
+  (*       (consSigs : Vector.t consSig n) *)
+  (*       (methSigs : Vector.t methSig n') *)
+  (*       (consDefs : ilist (B := @consDef Rep) consSigs) *)
+  (*       (methDefs : ilist (B := @methDef Rep) methSigs) *)
+  (*       (idx : @Fin.t n) *)
+  (*       (newDef : consDef (Vector.nth consSigs idx)) *)
+  (* : *)
+  (*   (forall consIdx, *)
+  (*      refineConstructor AbsR (getConsDef consDefs consIdx) (getConsDef consDefs consIdx)) *)
+  (*   -> (forall methIdx, *)
+  (*         refineMethod AbsR (getMethDef methDefs methIdx) (getMethDef methDefs methIdx)) *)
+  (*   -> refineConstructor AbsR *)
+  (*                        (consBody (ith consDefs idx )) *)
+  (*                        (consBody newDef) *)
+  (*   -> refineADT *)
+  (*        (BuildADT consDefs methDefs) *)
+  (*        (ADTReplaceConsDef consDefs methDefs idx newDef). *)
+  (* Proof. *)
+  (*   intros; eapply refineADT_BuildADT_Rep with (AbsR := AbsR); eauto. *)
+  (*   intros; unfold getConsDef. *)
+  (*   unfold replaceConsDef. *)
+  (*   destruct (fin_eq_dec consIdx idx); subst. *)
+  (*   rewrite ith_replace_Index_eq; eauto. *)
+  (*   rewrite ith_replace_Index_neq; eauto. *)
+  (* Qed. *)
 
-  Corollary SharpenStep_BuildADT_ReplaceConstructor_eq
-            (Rep : Type)
-            {n n'}
-            (consSigs : Vector.t consSig n)
-            (methSigs : Vector.t methSig n')
-            (consDefs : ilist (B := @consDef Rep) consSigs)
-            (methDefs : ilist (B := @methDef Rep) methSigs)
-            (idx : @Fin.t n)
-            (newDef : consDef (Vector.nth consSigs idx))
-            adt''
-    :
-    (let H := consBody newDef in refineConstructor eq (consBody (ith consDefs idx)) H)
-    -> refineADT (ADTReplaceConsDef consDefs methDefs idx newDef) adt''
-    -> refineADT (BuildADT consDefs methDefs) adt''.
-  Proof.
-    intros; eapply SharpenStep; try exact X.
-    eapply refineADT_BuildADT_ReplaceConstructor with (AbsR := eq);
-    simpl; unfold refine; intros; subst; eauto.
-    - reflexivity.
-    - reflexivity.
-  Qed.
+  (* Corollary SharpenStep_BuildADT_ReplaceConstructor_eq *)
+  (*           (Rep : Type) *)
+  (*           {n n'} *)
+  (*           (consSigs : Vector.t consSig n) *)
+  (*           (methSigs : Vector.t methSig n') *)
+  (*           (consDefs : ilist (B := @consDef Rep) consSigs) *)
+  (*           (methDefs : ilist (B := @methDef Rep) methSigs) *)
+  (*           (idx : @Fin.t n) *)
+  (*           (newDef : consDef (Vector.nth consSigs idx)) *)
+  (*           adt'' *)
+  (*   : *)
+  (*   (let H := consBody newDef in refineConstructor eq (consBody (ith consDefs idx)) H) *)
+  (*   -> refineADT (ADTReplaceConsDef consDefs methDefs idx newDef) adt'' *)
+  (*   -> refineADT (BuildADT consDefs methDefs) adt''. *)
+  (* Proof. *)
+  (*   intros; eapply SharpenStep; try exact X. *)
+  (*   eapply refineADT_BuildADT_ReplaceConstructor with (AbsR := eq); *)
+  (*   simpl; unfold refine; intros; subst; eauto. *)
+  (*   - reflexivity. *)
+  (*   - reflexivity. *)
+  (* Qed. *)
 
-  Corollary FullySharpenStep_BuildADT_ReplaceConstructor_eq
-            (Rep : Type)
-            {n n'}
-            (consSigs : Vector.t consSig n)
-            (methSigs : Vector.t methSig n')
-            (consDefs : ilist (B := @consDef Rep) consSigs)
-            (methDefs : ilist (B := @methDef Rep) methSigs)
-            (idx : @Fin.t n)
-            (newDef : consDef (Vector.nth consSigs idx))
-            adt''
-    :
-      (let H := consBody newDef in refineConstructor eq (consBody (ith consDefs idx)) H)
-    -> FullySharpenedUnderDelegates (ADTReplaceConsDef consDefs methDefs idx newDef) adt''
-    -> FullySharpenedUnderDelegates (BuildADT consDefs methDefs) adt''.
-  Proof.
-    intros; eapply FullySharpenStep; try exact X.
-    eapply refineADT_BuildADT_ReplaceConstructor with (AbsR := eq);
-    simpl; unfold refine; intros; subst; eauto.
-    - reflexivity.
-    - reflexivity.
-  Qed.
+  (* Corollary FullySharpenStep_BuildADT_ReplaceConstructor_eq *)
+  (*           (Rep : Type) *)
+  (*           {n n'} *)
+  (*           (consSigs : Vector.t consSig n) *)
+  (*           (methSigs : Vector.t methSig n') *)
+  (*           (consDefs : ilist (B := @consDef Rep) consSigs) *)
+  (*           (methDefs : ilist (B := @methDef Rep) methSigs) *)
+  (*           (idx : @Fin.t n) *)
+  (*           (newDef : consDef (Vector.nth consSigs idx)) *)
+  (*           adt'' *)
+  (*   : *)
+  (*     (let H := consBody newDef in refineConstructor eq (consBody (ith consDefs idx)) H) *)
+  (*   -> FullySharpenedUnderDelegates (ADTReplaceConsDef consDefs methDefs idx newDef) adt'' *)
+  (*   -> FullySharpenedUnderDelegates (BuildADT consDefs methDefs) adt''. *)
+  (* Proof. *)
+  (*   intros; eapply FullySharpenStep; try exact X. *)
+  (*   eapply refineADT_BuildADT_ReplaceConstructor with (AbsR := eq); *)
+  (*   simpl; unfold refine; intros; subst; eauto. *)
+  (*   - reflexivity. *)
+  (*   - reflexivity. *)
+  (* Qed. *)
 
   (* Corollary SharpenStep_BuildADT_ReplaceConstructor_eq
             (Rep : Type)
@@ -191,82 +191,82 @@ Lemma refineADT_BuildADT_ReplaceConstructor_sigma
       assumption.
   Qed. *)
 
-  Lemma refineADT_BuildADT_ReplaceMethod
-        (Rep : Type)
-        {n n'}
-        (consSigs : Vector.t consSig n)
-        (methSigs : Vector.t methSig n')
-        (consDefs : ilist (B := @consDef Rep) consSigs)
-        (methDefs : ilist (B := @methDef Rep) methSigs)
-        (idx : @Fin.t n')
-        (newDef : methDef (Vector.nth methSigs idx))
-        AbsR
-        (AbsR_reflexive_constructor :
-           forall consIdx,
-             refineConstructor AbsR (getConsDef consDefs consIdx) (getConsDef consDefs consIdx))
-        (AbsR_reflexive_method :
-           forall methIdx,
-             refineMethod AbsR (getMethDef methDefs methIdx) (getMethDef methDefs methIdx))
-  : refineMethod AbsR
-                 (methBody (ith methDefs idx))
-                 (methBody newDef)
-    -> refineADT
-         (BuildADT consDefs methDefs)
-         (ADTReplaceMethDef consDefs methDefs idx newDef).
-  Proof.
-    intros; eapply refineADT_BuildADT_Rep with (AbsR := AbsR); trivial.
-    intros; unfold getMethDef.
-    unfold replaceMethDef.
-    destruct (fin_eq_dec methIdx idx); subst.
-    rewrite ith_replace_Index_eq; eauto.
-    rewrite ith_replace_Index_neq; eauto.
-  Qed.
+  (* Lemma refineADT_BuildADT_ReplaceMethod *)
+  (*       (Rep : Type) *)
+  (*       {n n'} *)
+  (*       (consSigs : Vector.t consSig n) *)
+  (*       (methSigs : Vector.t methSig n') *)
+  (*       (consDefs : ilist (B := @consDef Rep) consSigs) *)
+  (*       (methDefs : ilist (B := @methDef Rep) methSigs) *)
+  (*       (idx : @Fin.t n') *)
+  (*       (newDef : methDef (Vector.nth methSigs idx)) *)
+  (*       AbsR *)
+  (*       (AbsR_reflexive_constructor : *)
+  (*          forall consIdx, *)
+  (*            refineConstructor AbsR (getConsDef consDefs consIdx) (getConsDef consDefs consIdx)) *)
+  (*       (AbsR_reflexive_method : *)
+  (*          forall methIdx, *)
+  (*            refineMethod AbsR (getMethDef methDefs methIdx) (getMethDef methDefs methIdx)) *)
+  (* : refineMethod AbsR *)
+  (*                (methBody (ith methDefs idx)) *)
+  (*                (methBody newDef) *)
+  (*   -> refineADT *)
+  (*        (BuildADT consDefs methDefs) *)
+  (*        (ADTReplaceMethDef consDefs methDefs idx newDef). *)
+  (* Proof. *)
+  (*   intros; eapply refineADT_BuildADT_Rep with (AbsR := AbsR); trivial. *)
+  (*   intros; unfold getMethDef. *)
+  (*   unfold replaceMethDef. *)
+  (*   destruct (fin_eq_dec methIdx idx); subst. *)
+  (*   rewrite ith_replace_Index_eq; eauto. *)
+  (*   rewrite ith_replace_Index_neq; eauto. *)
+  (* Qed. *)
 
-  Corollary SharpenStep_BuildADT_ReplaceMethod_eq
-        (Rep : Type)
-        {n n'}
-        (consSigs : Vector.t consSig n)
-        (methSigs : Vector.t methSig n')
-        (consDefs : ilist (B := @consDef Rep) consSigs)
-        (methDefs : ilist (B := @methDef Rep) methSigs)
-        (idx : @Fin.t n')
-        (newDef : methDef (Vector.nth methSigs idx))
-        adt''
-    :
-      (let H := methBody newDef in refineMethod eq (methBody (ith methDefs idx)) newDef)
-      -> refineADT (ADTReplaceMethDef consDefs methDefs idx newDef) adt''
-      -> refineADT (BuildADT consDefs methDefs) adt''.
-  Proof.
-    intros; eapply SharpenStep.
-    eapply refineADT_BuildADT_ReplaceMethod with (AbsR := eq);
-    simpl; unfold refine; intros; subst; eauto; reflexivity.
-    exact X.
-  Qed.
+  (* Corollary SharpenStep_BuildADT_ReplaceMethod_eq *)
+  (*       (Rep : Type) *)
+  (*       {n n'} *)
+  (*       (consSigs : Vector.t consSig n) *)
+  (*       (methSigs : Vector.t methSig n') *)
+  (*       (consDefs : ilist (B := @consDef Rep) consSigs) *)
+  (*       (methDefs : ilist (B := @methDef Rep) methSigs) *)
+  (*       (idx : @Fin.t n') *)
+  (*       (newDef : methDef (Vector.nth methSigs idx)) *)
+  (*       adt'' *)
+  (*   : *)
+  (*     (let H := methBody newDef in refineMethod eq (methBody (ith methDefs idx)) newDef) *)
+  (*     -> refineADT (ADTReplaceMethDef consDefs methDefs idx newDef) adt'' *)
+  (*     -> refineADT (BuildADT consDefs methDefs) adt''. *)
+  (* Proof. *)
+  (*   intros; eapply SharpenStep. *)
+  (*   eapply refineADT_BuildADT_ReplaceMethod with (AbsR := eq); *)
+  (*   simpl; unfold refine; intros; subst; eauto; reflexivity. *)
+  (*   exact X. *)
+  (* Qed. *)
 
-  Lemma FullySharpenStep_BuildADT_ReplaceMethod_eq
-        (Rep : Type)
-        {n n'}
-        (consSigs : Vector.t consSig n)
-        (methSigs : Vector.t methSig n')
-        (consDefs : ilist (B := @consDef Rep) consSigs)
-        (methDefs : ilist (B := @methDef Rep) methSigs)
-        (idx : @Fin.t n')
-        (newDef : methDef (Vector.nth methSigs idx))
-        adt''
-    :
-      (let H := methBody newDef in refineMethod eq (methBody (ith methDefs idx)) newDef)
-      -> FullySharpenedUnderDelegates
-           (ADTReplaceMethDef consDefs methDefs idx newDef)
-           adt''
-      -> FullySharpenedUnderDelegates
-           (BuildADT consDefs methDefs)
-           adt''.
-  Proof.
-    intros; eapply FullySharpenStep.
-    eapply refineADT_BuildADT_ReplaceMethod with (AbsR := eq);
-    simpl; unfold refine; intros; subst; eauto; reflexivity.
-    exact X.
-  Qed.
+  (* Lemma FullySharpenStep_BuildADT_ReplaceMethod_eq *)
+  (*       (Rep : Type) *)
+  (*       {n n'} *)
+  (*       (consSigs : Vector.t consSig n) *)
+  (*       (methSigs : Vector.t methSig n') *)
+  (*       (consDefs : ilist (B := @consDef Rep) consSigs) *)
+  (*       (methDefs : ilist (B := @methDef Rep) methSigs) *)
+  (*       (idx : @Fin.t n') *)
+  (*       (newDef : methDef (Vector.nth methSigs idx)) *)
+  (*       adt'' *)
+  (*   : *)
+  (*     (let H := methBody newDef in refineMethod eq (methBody (ith methDefs idx)) newDef) *)
+  (*     -> FullySharpenedUnderDelegates *)
+  (*          (ADTReplaceMethDef consDefs methDefs idx newDef) *)
+  (*          adt'' *)
+  (*     -> FullySharpenedUnderDelegates *)
+  (*          (BuildADT consDefs methDefs) *)
+  (*          adt''. *)
+  (* Proof. *)
+  (*   intros; eapply FullySharpenStep. *)
+  (*   eapply refineADT_BuildADT_ReplaceMethod with (AbsR := eq); *)
+  (*   simpl; unfold refine; intros; subst; eauto; reflexivity. *)
+  (*   exact X. *)
+  (* Qed. *)
 
   (*Corollary SharpenStep_BuildADT_ReplaceMethod_eq *)
 (*             (Rep : Type) *)
@@ -318,391 +318,391 @@ Lemma refineADT_BuildADT_ReplaceConstructor_sigma
   (* Notation-Friendly Lemmas for constructing an easily extractible *)
 (*      ADT implementation. *)
 
-  Definition Notation_Friendly_BuildMostlySharpenedcADT
-             {n n'}
-             {consSigs : Vector.t consSig n}
-             {methSigs : Vector.t methSig n'}
-             (DelegateIDs : nat)
-             (DelegateSigs : Fin.t DelegateIDs -> ADTSig)
-             (rep : (Fin.t DelegateIDs -> Type) -> Type)
-             (cConstructors :
-                forall
-                  (DelegateReps : Fin.t DelegateIDs -> Type)
-                  (DelegateImpls : forall idx,
-                                     ComputationalADT.pcADT (DelegateSigs idx) (DelegateReps idx)),
-                  ilist
-                    (B := fun Sig : consSig =>
-                            ComputationalADT.cConstructorType (rep DelegateReps) (consDom Sig))
-                    consSigs)
-             (cMethods :
-                forall
-                  (DelegateReps : Fin.t DelegateIDs -> Type)
-                  (DelegateImpls : forall idx,
-                                     ComputationalADT.pcADT (DelegateSigs idx) (DelegateReps idx)),
-                  ilist
-                    (B := fun Sig : methSig =>
-                       ComputationalADT.cMethodType (rep DelegateReps)
-                                                    (methDom Sig) (methCod Sig)) methSigs)
-             (DelegateReps : Fin.t DelegateIDs -> Type)
-             (DelegateImpls : forall idx,
-                                ComputationalADT.pcADT (DelegateSigs idx) (DelegateReps idx))
-  : ComputationalADT.cADT (BuildADTSig consSigs methSigs) :=
-    BuildcADT
-      (imap (Build_cConsDef (rep DelegateReps))
-            (cConstructors DelegateReps DelegateImpls))
-      (imap (Build_cMethDef (Rep:=rep DelegateReps))
-            (cMethods DelegateReps DelegateImpls)).
+(*   Definition Notation_Friendly_BuildMostlySharpenedcADT *)
+(*              {n n'} *)
+(*              {consSigs : Vector.t consSig n} *)
+(*              {methSigs : Vector.t methSig n'} *)
+(*              (DelegateIDs : nat) *)
+(*              (DelegateSigs : Fin.t DelegateIDs -> ADTSig) *)
+(*              (rep : (Fin.t DelegateIDs -> Type) -> Type) *)
+(*              (cConstructors : *)
+(*                 forall *)
+(*                   (DelegateReps : Fin.t DelegateIDs -> Type) *)
+(*                   (DelegateImpls : forall idx, *)
+(*                                      ComputationalADT.pcADT (DelegateSigs idx) (DelegateReps idx)), *)
+(*                   ilist *)
+(*                     (B := fun Sig : consSig => *)
+(*                             ComputationalADT.cConstructorType (rep DelegateReps) (consDom Sig)) *)
+(*                     consSigs) *)
+(*              (cMethods : *)
+(*                 forall *)
+(*                   (DelegateReps : Fin.t DelegateIDs -> Type) *)
+(*                   (DelegateImpls : forall idx, *)
+(*                                      ComputationalADT.pcADT (DelegateSigs idx) (DelegateReps idx)), *)
+(*                   ilist *)
+(*                     (B := fun Sig : methSig => *)
+(*                        ComputationalADT.cMethodType (rep DelegateReps) *)
+(*                                                     (methDom Sig) (methCod Sig)) methSigs) *)
+(*              (DelegateReps : Fin.t DelegateIDs -> Type) *)
+(*              (DelegateImpls : forall idx, *)
+(*                                 ComputationalADT.pcADT (DelegateSigs idx) (DelegateReps idx)) *)
+(*   : ComputationalADT.cADT (BuildADTSig consSigs methSigs) := *)
+(*     BuildcADT *)
+(*       (imap (Build_cConsDef (rep DelegateReps)) *)
+(*             (cConstructors DelegateReps DelegateImpls)) *)
+(*       (imap (Build_cMethDef (Rep:=rep DelegateReps)) *)
+(*             (cMethods DelegateReps DelegateImpls)). *)
 
-  Definition Notation_Friendly_FullySharpened_BuildMostlySharpenedcADT
-             (RepT : Type)
-             {n n'}
-             {consSigs : Vector.t consSig n}
-             {methSigs : Vector.t methSig n'}
-             (consDefs : ilist consSigs)
-             (methDefs : ilist methSigs)
-             (DelegateIDs : nat)
-             (DelegateSigs : Fin.t DelegateIDs -> ADTSig)
-             (rep : (Fin.t DelegateIDs -> Type) -> Type)
-             (cConstructors :
-                forall
-                  (DelegateReps : Fin.t DelegateIDs -> Type)
-                  (DelegateImpls : forall idx,
-                                     ComputationalADT.pcADT (DelegateSigs idx) (DelegateReps idx)),
-                  ilist
-                    (B := fun Sig : consSig =>
-                       ComputationalADT.cConstructorType
-                         (rep DelegateReps) (consDom Sig)) consSigs)
-             (cMethods :
-                forall
-                  (DelegateReps : Fin.t DelegateIDs -> Type)
-                  (DelegateImpls : forall idx,
-                                     ComputationalADT.pcADT (DelegateSigs idx) (DelegateReps idx)),
-                  ilist
-                    (B := fun Sig : methSig =>
-                       ComputationalADT.cMethodType
-                         (rep DelegateReps) (methDom Sig)
-                         (methCod Sig)) methSigs)
-             (DelegateSpecs : forall idx, ADT (DelegateSigs idx))
-             (cAbsR :
-                forall
-                  (DelegateReps : Fin.t DelegateIDs -> Type)
-                  (DelegateImpls : forall idx,
-                                     ComputationalADT.pcADT (DelegateSigs idx) (DelegateReps idx))
-                  (ValidImpls
-                   : forall idx : Fin.t DelegateIDs,
-                       refineADT (DelegateSpecs idx)
-                                 (ComputationalADT.LiftcADT (existT _ _ (DelegateImpls idx)))),
-                  RepT -> rep DelegateReps -> Prop)
-             (cConstructorsRefinesSpec : forall
-                                           (DelegateReps : Fin.t DelegateIDs -> Type)
-                                           (DelegateImpls : forall idx,
-                                                              ComputationalADT.pcADT (DelegateSigs idx) (DelegateReps idx))
-                                           (ValidImpls
-                                            : forall idx : Fin.t DelegateIDs,
-                                                refineADT (DelegateSpecs idx)
-                                                          (ComputationalADT.LiftcADT (existT _ _ (DelegateImpls idx)))),
-                 Iterate_Dep_Type_BoundedIndex
-                   (fun idx  =>
-                      @refineConstructor
-                        (RepT) (rep DelegateReps) (cAbsR _ _ ValidImpls)
-                        (consDom (Vector.nth consSigs idx))
-                        (getConsDef consDefs idx)
-                        (LiftcConstructor _ _ (ith (cConstructors DelegateReps DelegateImpls) idx))))
-             (cMethodsRefinesSpec : forall
-                                      (DelegateReps : Fin.t DelegateIDs -> Type)
-                                      (DelegateImpls : forall idx,
-                                                         ComputationalADT.pcADT (DelegateSigs idx) (DelegateReps idx))
-                                      (ValidImpls
-                                       : forall idx : Fin.t DelegateIDs,
-                                           refineADT (DelegateSpecs idx)
-                                                     (ComputationalADT.LiftcADT (existT _ _ (DelegateImpls idx)))),
-                                      Iterate_Dep_Type_BoundedIndex
-                                        (fun idx =>
-                                           @refineMethod
-                                             RepT (rep DelegateReps)
-                                             (cAbsR _ _ ValidImpls)
-                                             (methDom (Vector.nth methSigs idx))
-                                             (methCod (Vector.nth methSigs idx))
-                                             (getMethDef methDefs idx)
-                                             (LiftcMethod (ith (cMethods DelegateReps DelegateImpls) idx))))
-  : FullySharpenedUnderDelegates (BuildADT consDefs methDefs)
-                                 {|
-                                   Sharpened_DelegateSigs := DelegateSigs;
-                                   Sharpened_Implementation := Notation_Friendly_BuildMostlySharpenedcADT
-                                                                 _ rep cConstructors cMethods;
-                                   Sharpened_DelegateSpecs := DelegateSpecs |}.
-  Proof.
-    intros * DelegateReps DelegateImpls DelegateImplRefinesSpec.
-    eapply (@refinesADT _ (BuildADT consDefs methDefs)
-                        (LiftcADT (existT _ (rep DelegateReps)
-                                          {| pcConstructors := _;
-                                             pcMethods := _|}))
-                        (cAbsR DelegateReps DelegateImpls DelegateImplRefinesSpec)).
-    - simpl; unfold ComputationalADT.cConstructors; simpl; intros.
-      rewrite <- ith_imap; eauto.
-      apply (Lookup_Iterate_Dep_Type
-                 _ (cConstructorsRefinesSpec DelegateReps DelegateImpls DelegateImplRefinesSpec) idx).
-        (*as [c [AbsR_c computes_c] ]. *)
-(*       unfold refine; intros; inversion_by computes_to_inv; subst. *)
-(*       econstructor; eauto. *)
-    - simpl; unfold ComputationalADT.cMethods; simpl; intros.
-      rewrite <- ith_imap.
-      apply (Lookup_Iterate_Dep_Type
-                  _ (cMethodsRefinesSpec DelegateReps DelegateImpls DelegateImplRefinesSpec)).
-        (* as [r_o' [AbsR_r_o' computes_r_o'] ]. *)
-(*       unfold refine; intros; inversion_by computes_to_inv; subst; *)
-(*       econstructor; eauto. *)
-(*       econstructor; eauto. *)
-(*       case_eq ((ith_Bounded methID (cMethods DelegateReps DelegateImpls) idx r_n d)); *)
-(*         simpl; intros; eauto. *)
-(*       rewrite H0; eauto. *)
-  Qed.
+(*   Definition Notation_Friendly_FullySharpened_BuildMostlySharpenedcADT *)
+(*              (RepT : Type) *)
+(*              {n n'} *)
+(*              {consSigs : Vector.t consSig n} *)
+(*              {methSigs : Vector.t methSig n'} *)
+(*              (consDefs : ilist consSigs) *)
+(*              (methDefs : ilist methSigs) *)
+(*              (DelegateIDs : nat) *)
+(*              (DelegateSigs : Fin.t DelegateIDs -> ADTSig) *)
+(*              (rep : (Fin.t DelegateIDs -> Type) -> Type) *)
+(*              (cConstructors : *)
+(*                 forall *)
+(*                   (DelegateReps : Fin.t DelegateIDs -> Type) *)
+(*                   (DelegateImpls : forall idx, *)
+(*                                      ComputationalADT.pcADT (DelegateSigs idx) (DelegateReps idx)), *)
+(*                   ilist *)
+(*                     (B := fun Sig : consSig => *)
+(*                        ComputationalADT.cConstructorType *)
+(*                          (rep DelegateReps) (consDom Sig)) consSigs) *)
+(*              (cMethods : *)
+(*                 forall *)
+(*                   (DelegateReps : Fin.t DelegateIDs -> Type) *)
+(*                   (DelegateImpls : forall idx, *)
+(*                                      ComputationalADT.pcADT (DelegateSigs idx) (DelegateReps idx)), *)
+(*                   ilist *)
+(*                     (B := fun Sig : methSig => *)
+(*                        ComputationalADT.cMethodType *)
+(*                          (rep DelegateReps) (methDom Sig) *)
+(*                          (methCod Sig)) methSigs) *)
+(*              (DelegateSpecs : forall idx, ADT (DelegateSigs idx)) *)
+(*              (cAbsR : *)
+(*                 forall *)
+(*                   (DelegateReps : Fin.t DelegateIDs -> Type) *)
+(*                   (DelegateImpls : forall idx, *)
+(*                                      ComputationalADT.pcADT (DelegateSigs idx) (DelegateReps idx)) *)
+(*                   (ValidImpls *)
+(*                    : forall idx : Fin.t DelegateIDs, *)
+(*                        refineADT (DelegateSpecs idx) *)
+(*                                  (ComputationalADT.LiftcADT (existT _ _ (DelegateImpls idx)))), *)
+(*                   RepT -> rep DelegateReps -> Prop) *)
+(*              (cConstructorsRefinesSpec : forall *)
+(*                                            (DelegateReps : Fin.t DelegateIDs -> Type) *)
+(*                                            (DelegateImpls : forall idx, *)
+(*                                                               ComputationalADT.pcADT (DelegateSigs idx) (DelegateReps idx)) *)
+(*                                            (ValidImpls *)
+(*                                             : forall idx : Fin.t DelegateIDs, *)
+(*                                                 refineADT (DelegateSpecs idx) *)
+(*                                                           (ComputationalADT.LiftcADT (existT _ _ (DelegateImpls idx)))), *)
+(*                  Iterate_Dep_Type_BoundedIndex *)
+(*                    (fun idx  => *)
+(*                       @refineConstructor *)
+(*                         (RepT) (rep DelegateReps) (cAbsR _ _ ValidImpls) *)
+(*                         (consDom (Vector.nth consSigs idx)) *)
+(*                         (getConsDef consDefs idx) *)
+(*                         (LiftcConstructor _ _ (ith (cConstructors DelegateReps DelegateImpls) idx)))) *)
+(*              (cMethodsRefinesSpec : forall *)
+(*                                       (DelegateReps : Fin.t DelegateIDs -> Type) *)
+(*                                       (DelegateImpls : forall idx, *)
+(*                                                          ComputationalADT.pcADT (DelegateSigs idx) (DelegateReps idx)) *)
+(*                                       (ValidImpls *)
+(*                                        : forall idx : Fin.t DelegateIDs, *)
+(*                                            refineADT (DelegateSpecs idx) *)
+(*                                                      (ComputationalADT.LiftcADT (existT _ _ (DelegateImpls idx)))), *)
+(*                                       Iterate_Dep_Type_BoundedIndex *)
+(*                                         (fun idx => *)
+(*                                            @refineMethod *)
+(*                                              RepT (rep DelegateReps) *)
+(*                                              (cAbsR _ _ ValidImpls) *)
+(*                                              (methDom (Vector.nth methSigs idx)) *)
+(*                                              (methCod (Vector.nth methSigs idx)) *)
+(*                                              (getMethDef methDefs idx) *)
+(*                                              (LiftcMethod (ith (cMethods DelegateReps DelegateImpls) idx)))) *)
+(*   : FullySharpenedUnderDelegates (BuildADT consDefs methDefs) *)
+(*                                  {| *)
+(*                                    Sharpened_DelegateSigs := DelegateSigs; *)
+(*                                    Sharpened_Implementation := Notation_Friendly_BuildMostlySharpenedcADT *)
+(*                                                                  _ rep cConstructors cMethods; *)
+(*                                    Sharpened_DelegateSpecs := DelegateSpecs |}. *)
+(*   Proof. *)
+(*     intros * DelegateReps DelegateImpls DelegateImplRefinesSpec. *)
+(*     eapply (@refinesADT _ (BuildADT consDefs methDefs) *)
+(*                         (LiftcADT (existT _ (rep DelegateReps) *)
+(*                                           {| pcConstructors := _; *)
+(*                                              pcMethods := _|})) *)
+(*                         (cAbsR DelegateReps DelegateImpls DelegateImplRefinesSpec)). *)
+(*     - simpl; unfold ComputationalADT.cConstructors; simpl; intros. *)
+(*       rewrite <- ith_imap; eauto. *)
+(*       apply (Lookup_Iterate_Dep_Type *)
+(*                  _ (cConstructorsRefinesSpec DelegateReps DelegateImpls DelegateImplRefinesSpec) idx). *)
+(*         (*as [c [AbsR_c computes_c] ]. *) *)
+(* (*       unfold refine; intros; inversion_by computes_to_inv; subst. *) *)
+(* (*       econstructor; eauto. *) *)
+(*     - simpl; unfold ComputationalADT.cMethods; simpl; intros. *)
+(*       rewrite <- ith_imap. *)
+(*       apply (Lookup_Iterate_Dep_Type *)
+(*                   _ (cMethodsRefinesSpec DelegateReps DelegateImpls DelegateImplRefinesSpec)). *)
+(*         (* as [r_o' [AbsR_r_o' computes_r_o'] ]. *) *)
+(* (*       unfold refine; intros; inversion_by computes_to_inv; subst; *) *)
+(* (*       econstructor; eauto. *) *)
+(* (*       econstructor; eauto. *) *)
+(* (*       case_eq ((ith_Bounded methID (cMethods DelegateReps DelegateImpls) idx r_n d)); *) *)
+(* (*         simpl; intros; eauto. *) *)
+(* (*       rewrite H0; eauto. *) *)
+(*   Qed. *)
 
-  Definition Notation_Friendly_SharpenFully'
-             (RepT : Type)
-             {n n'}
-             (consSigs : Vector.t consSig n)
-             (methSigs : Vector.t methSig n')
-             (consDefs : ilist consSigs)
-             (methDefs : ilist methSigs)
-             (DelegateIDs : nat)
-             (DelegateSigs : Fin.t DelegateIDs -> ADTSig)
-             (rep : (Fin.t DelegateIDs -> Type) -> Type)
-             (cConstructors :
-                forall
-                  (DelegateReps : Fin.t DelegateIDs -> Type)
-                  (DelegateImpls : forall idx,
-                                     ComputationalADT.pcADT (DelegateSigs idx) (DelegateReps idx)),
-                  ilist
-                    (B := fun Sig : consSig =>
-                       ComputationalADT.cConstructorType
-                         (rep DelegateReps) (consDom Sig)) consSigs)
-             (cMethods :
-                forall
-                  (DelegateReps : Fin.t DelegateIDs -> Type)
-                  (DelegateImpls : forall idx,
-                                     ComputationalADT.pcADT (DelegateSigs idx) (DelegateReps idx)),
-                  ilist
-                    (B := fun Sig : methSig =>
-                       ComputationalADT.cMethodType
-                         (rep DelegateReps) (methDom Sig)
-                         (methCod Sig)) methSigs)
-             (DelegateSpecs : forall idx, ADT (DelegateSigs idx))
-             (cAbsR :
-                forall
-                  (DelegateReps : Fin.t DelegateIDs -> Type)
-                  (DelegateImpls : forall idx,
-                                     ComputationalADT.pcADT (DelegateSigs idx) (DelegateReps idx))
-                  (ValidImpls
-                   : forall idx : Fin.t DelegateIDs,
-                       refineADT (DelegateSpecs idx)
-                                 (ComputationalADT.LiftcADT (existT _ _ (DelegateImpls idx)))),
-                  RepT -> rep DelegateReps -> Prop)
-             (cConstructorsRefinesSpec : forall
-                                           (DelegateReps : Fin.t DelegateIDs -> Type)
-                                           (DelegateImpls : forall idx,
-                                                              ComputationalADT.pcADT (DelegateSigs idx) (DelegateReps idx))
-                                           (ValidImpls
-                                            : forall idx : Fin.t DelegateIDs,
-                                                refineADT (DelegateSpecs idx)
-                                                          (ComputationalADT.LiftcADT (existT _ _ (DelegateImpls idx)))),
-                                           Iterate_Dep_Type_BoundedIndex
-                                             (fun idx  =>
-                                                @refineConstructor
-                                                  (RepT) (rep DelegateReps) (cAbsR _ _ ValidImpls)
-                                                  (consDom (Vector.nth consSigs idx))
-                                                  (getConsDef consDefs idx)
-                                                  (LiftcConstructor _ _ (ith (cConstructors DelegateReps DelegateImpls) idx))))
-             (cMethodsRefinesSpec : forall
-                                      (DelegateReps : Fin.t DelegateIDs -> Type)
-                                      (DelegateImpls : forall idx,
-                                                         ComputationalADT.pcADT (DelegateSigs idx) (DelegateReps idx))
-                                      (ValidImpls
-                                       : forall idx : Fin.t DelegateIDs,
-                                           refineADT (DelegateSpecs idx)
-                                                     (ComputationalADT.LiftcADT (existT _ _ (DelegateImpls idx)))),
-                                      Iterate_Dep_Type_BoundedIndex
-                                        (fun idx  =>
-                                           @refineMethod
-                                             RepT (rep DelegateReps)
-                                             (cAbsR _ _ ValidImpls)
-                                             (methDom (Vector.nth methSigs idx))
-                                             (methCod (Vector.nth methSigs idx))
-                                             (getMethDef methDefs idx)
-                                             (LiftcMethod (ith (cMethods DelegateReps DelegateImpls) idx ))))
-  : FullySharpenedUnderDelegates
-      (BuildADT consDefs methDefs)
-      {|
-        Sharpened_DelegateSigs := DelegateSigs;
-        Sharpened_Implementation := Notation_Friendly_BuildMostlySharpenedcADT _ rep
-                                                                               cConstructors cMethods;
-        Sharpened_DelegateSpecs := DelegateSpecs |} :=
-                                 (Notation_Friendly_FullySharpened_BuildMostlySharpenedcADT consDefs
-                                                                      methDefs _ rep cConstructors cMethods DelegateSpecs cAbsR
-                                                                      cConstructorsRefinesSpec cMethodsRefinesSpec).
+(*   Definition Notation_Friendly_SharpenFully' *)
+(*              (RepT : Type) *)
+(*              {n n'} *)
+(*              (consSigs : Vector.t consSig n) *)
+(*              (methSigs : Vector.t methSig n') *)
+(*              (consDefs : ilist consSigs) *)
+(*              (methDefs : ilist methSigs) *)
+(*              (DelegateIDs : nat) *)
+(*              (DelegateSigs : Fin.t DelegateIDs -> ADTSig) *)
+(*              (rep : (Fin.t DelegateIDs -> Type) -> Type) *)
+(*              (cConstructors : *)
+(*                 forall *)
+(*                   (DelegateReps : Fin.t DelegateIDs -> Type) *)
+(*                   (DelegateImpls : forall idx, *)
+(*                                      ComputationalADT.pcADT (DelegateSigs idx) (DelegateReps idx)), *)
+(*                   ilist *)
+(*                     (B := fun Sig : consSig => *)
+(*                        ComputationalADT.cConstructorType *)
+(*                          (rep DelegateReps) (consDom Sig)) consSigs) *)
+(*              (cMethods : *)
+(*                 forall *)
+(*                   (DelegateReps : Fin.t DelegateIDs -> Type) *)
+(*                   (DelegateImpls : forall idx, *)
+(*                                      ComputationalADT.pcADT (DelegateSigs idx) (DelegateReps idx)), *)
+(*                   ilist *)
+(*                     (B := fun Sig : methSig => *)
+(*                        ComputationalADT.cMethodType *)
+(*                          (rep DelegateReps) (methDom Sig) *)
+(*                          (methCod Sig)) methSigs) *)
+(*              (DelegateSpecs : forall idx, ADT (DelegateSigs idx)) *)
+(*              (cAbsR : *)
+(*                 forall *)
+(*                   (DelegateReps : Fin.t DelegateIDs -> Type) *)
+(*                   (DelegateImpls : forall idx, *)
+(*                                      ComputationalADT.pcADT (DelegateSigs idx) (DelegateReps idx)) *)
+(*                   (ValidImpls *)
+(*                    : forall idx : Fin.t DelegateIDs, *)
+(*                        refineADT (DelegateSpecs idx) *)
+(*                                  (ComputationalADT.LiftcADT (existT _ _ (DelegateImpls idx)))), *)
+(*                   RepT -> rep DelegateReps -> Prop) *)
+(*              (cConstructorsRefinesSpec : forall *)
+(*                                            (DelegateReps : Fin.t DelegateIDs -> Type) *)
+(*                                            (DelegateImpls : forall idx, *)
+(*                                                               ComputationalADT.pcADT (DelegateSigs idx) (DelegateReps idx)) *)
+(*                                            (ValidImpls *)
+(*                                             : forall idx : Fin.t DelegateIDs, *)
+(*                                                 refineADT (DelegateSpecs idx) *)
+(*                                                           (ComputationalADT.LiftcADT (existT _ _ (DelegateImpls idx)))), *)
+(*                                            Iterate_Dep_Type_BoundedIndex *)
+(*                                              (fun idx  => *)
+(*                                                 @refineConstructor *)
+(*                                                   (RepT) (rep DelegateReps) (cAbsR _ _ ValidImpls) *)
+(*                                                   (consDom (Vector.nth consSigs idx)) *)
+(*                                                   (getConsDef consDefs idx) *)
+(*                                                   (LiftcConstructor _ _ (ith (cConstructors DelegateReps DelegateImpls) idx)))) *)
+(*              (cMethodsRefinesSpec : forall *)
+(*                                       (DelegateReps : Fin.t DelegateIDs -> Type) *)
+(*                                       (DelegateImpls : forall idx, *)
+(*                                                          ComputationalADT.pcADT (DelegateSigs idx) (DelegateReps idx)) *)
+(*                                       (ValidImpls *)
+(*                                        : forall idx : Fin.t DelegateIDs, *)
+(*                                            refineADT (DelegateSpecs idx) *)
+(*                                                      (ComputationalADT.LiftcADT (existT _ _ (DelegateImpls idx)))), *)
+(*                                       Iterate_Dep_Type_BoundedIndex *)
+(*                                         (fun idx  => *)
+(*                                            @refineMethod *)
+(*                                              RepT (rep DelegateReps) *)
+(*                                              (cAbsR _ _ ValidImpls) *)
+(*                                              (methDom (Vector.nth methSigs idx)) *)
+(*                                              (methCod (Vector.nth methSigs idx)) *)
+(*                                              (getMethDef methDefs idx) *)
+(*                                              (LiftcMethod (ith (cMethods DelegateReps DelegateImpls) idx )))) *)
+(*   : FullySharpenedUnderDelegates *)
+(*       (BuildADT consDefs methDefs) *)
+(*       {| *)
+(*         Sharpened_DelegateSigs := DelegateSigs; *)
+(*         Sharpened_Implementation := Notation_Friendly_BuildMostlySharpenedcADT _ rep *)
+(*                                                                                cConstructors cMethods; *)
+(*         Sharpened_DelegateSpecs := DelegateSpecs |} := *)
+(*                                  (Notation_Friendly_FullySharpened_BuildMostlySharpenedcADT consDefs *)
+(*                                                                       methDefs _ rep cConstructors cMethods DelegateSpecs cAbsR *)
+(*                                                                       cConstructorsRefinesSpec cMethodsRefinesSpec). *)
 
-  Record NamedDelegatee :=
-    { delegateeSig : ADTSig;
-      delegateeRep : Type }.
+(*   Record NamedDelegatee := *)
+(*     { delegateeSig : ADTSig; *)
+(*       delegateeRep : Type }. *)
 
-  Definition Build_NamedDelegatees
-           {n}
-           (DelegateSigs : Vector.t ADTSig n)
-           (DelegateReps : Vector.t Type n)
-  : Vector.t NamedDelegatee n.
-      pattern n, DelegateReps, DelegateSigs.
-      match goal with
-        |- ?P n DelegateReps DelegateSigs =>
-        simpl; refine (Vector.rect2
-                         P
-                         (Vector.nil _)
-                         (fun n DelegateReps DelegateSigs Delegatees Rep Sig =>
-                            (Vector.cons
-                               _
-                               {| delegateeSig := Sig; delegateeRep := Rep |}
-                               _ Delegatees))
-                         DelegateReps DelegateSigs)
-      end.
-  Defined.
+(*   Definition Build_NamedDelegatees *)
+(*            {n} *)
+(*            (DelegateSigs : Vector.t ADTSig n) *)
+(*            (DelegateReps : Vector.t Type n) *)
+(*   : Vector.t NamedDelegatee n. *)
+(*       pattern n, DelegateReps, DelegateSigs. *)
+(*       match goal with *)
+(*         |- ?P n DelegateReps DelegateSigs => *)
+(*         simpl; refine (Vector.rect2 *)
+(*                          P *)
+(*                          (Vector.nil _) *)
+(*                          (fun n DelegateReps DelegateSigs Delegatees Rep Sig => *)
+(*                             (Vector.cons *)
+(*                                _ *)
+(*                                {| delegateeSig := Sig; delegateeRep := Rep |} *)
+(*                                _ Delegatees)) *)
+(*                          DelegateReps DelegateSigs) *)
+(*       end. *)
+(*   Defined. *)
 
-  Definition Notation_Friendly_SharpenFully
-             (RepT : Type)
-             {m n n'}
-             (consSigs : Vector.t consSig n)
-             (methSigs : Vector.t methSig n')
-             (consDefs : ilist consSigs)
-             (methDefs : ilist methSigs)
-             (DelegateSigs' : Vector.t ADTSig m)
-             (DelegateReps' : Vector.t Type m)
-             (Delegatees := Build_NamedDelegatees DelegateSigs' DelegateReps')
-             (DelegateIDs := m)
-             (DelegateSigs := fun idx =>
-                                delegateeSig (Vector.nth Delegatees idx))
-             (DelegateReps := fun idx =>
-                                delegateeRep (Vector.nth Delegatees idx))
-             (rep : (Fin.t DelegateIDs -> Type) -> Type)
-             (cConstructors :
-                forall
-                  (DelegateReps : Fin.t DelegateIDs -> Type)
-                  (DelegateImpls : forall idx,
-                                     ComputationalADT.pcADT (DelegateSigs idx) (DelegateReps idx)),
-                  ilist
-                    (B := fun Sig : consSig =>
-                       ComputationalADT.cConstructorType
-                         (rep DelegateReps) (consDom Sig)) consSigs)
-             (cMethods :
-                forall
-                  (DelegateReps : Fin.t DelegateIDs -> Type)
-                  (DelegateImpls : forall idx,
-                                     ComputationalADT.pcADT (DelegateSigs idx) (DelegateReps idx)),
-                  ilist
-                    (B := fun Sig : methSig =>
-                       ComputationalADT.cMethodType
-                         (rep DelegateReps) (methDom Sig)
-                         (methCod Sig)) methSigs)
-             (DelegateSpecs' : ilist (B := fun nadt => ADT (delegateeSig nadt)) Delegatees )
-             (DelegateSpecs := ith DelegateSpecs')
-             (cAbsR :
-                forall
-                  (DelegateReps : Fin.t DelegateIDs -> Type)
-                  (DelegateImpls : forall idx,
-                                     ComputationalADT.pcADT (DelegateSigs idx) (DelegateReps idx))
-                  (ValidImpls
-                   : forall idx : Fin.t DelegateIDs,
-                       refineADT (DelegateSpecs idx)
-                                 (ComputationalADT.LiftcADT (existT _ _ (DelegateImpls idx)))),
-                  RepT -> rep DelegateReps -> Prop)
-             (cConstructorsRefinesSpec : forall
-                                           (DelegateReps : Fin.t DelegateIDs -> Type)
-                                           (DelegateImpls : forall idx,
-                                                              ComputationalADT.pcADT (DelegateSigs idx) (DelegateReps idx))
-                                           (ValidImpls
-                                            : forall idx : Fin.t DelegateIDs,
-                                                refineADT (DelegateSpecs idx)
-                                                          (ComputationalADT.LiftcADT (existT _ _ (DelegateImpls idx)))),
-                                           Iterate_Dep_Type_BoundedIndex
-                                             (fun idx =>
-                                                @refineConstructor
-                                                  (RepT) (rep DelegateReps) (cAbsR _ _ ValidImpls)
-                                                  (consDom (Vector.nth consSigs idx))
-                                                  (getConsDef consDefs idx)
-                                                  (LiftcConstructor _ _ (ith (cConstructors DelegateReps DelegateImpls) idx))))
-             (cMethodsRefinesSpec : forall
-                                      (DelegateReps : Fin.t DelegateIDs -> Type)
-                                      (DelegateImpls : forall idx,
-                                                         ComputationalADT.pcADT (DelegateSigs idx) (DelegateReps idx))
-                                      (ValidImpls
-                                       : forall idx : Fin.t DelegateIDs,
-                                           refineADT (DelegateSpecs idx)
-                                                     (ComputationalADT.LiftcADT (existT _ _ (DelegateImpls idx)))),
-                                      Iterate_Dep_Type_BoundedIndex
-                                        (fun idx =>
-                                           @refineMethod
-                                             RepT (rep DelegateReps)
-                                             (cAbsR _ _ ValidImpls)
-                                             (methDom (Vector.nth methSigs idx))
-                                             (methCod (Vector.nth methSigs idx))
-                                             (getMethDef methDefs idx)
-                                             (LiftcMethod (ith (cMethods DelegateReps DelegateImpls) idx))))
-  : FullySharpenedUnderDelegates
-      (BuildADT consDefs methDefs)
-      {|
-        Sharpened_DelegateSigs := DelegateSigs;
-        Sharpened_Implementation := Notation_Friendly_BuildMostlySharpenedcADT _ rep
-                                                                               cConstructors cMethods;
-        Sharpened_DelegateSpecs := DelegateSpecs |}.
-      refine (Notation_Friendly_FullySharpened_BuildMostlySharpenedcADT consDefs
-                                                                      methDefs _ rep cConstructors cMethods DelegateSpecs cAbsR
-                                                                      cConstructorsRefinesSpec cMethodsRefinesSpec).
-  Defined.
+(*   Definition Notation_Friendly_SharpenFully *)
+(*              (RepT : Type) *)
+(*              {m n n'} *)
+(*              (consSigs : Vector.t consSig n) *)
+(*              (methSigs : Vector.t methSig n') *)
+(*              (consDefs : ilist consSigs) *)
+(*              (methDefs : ilist methSigs) *)
+(*              (DelegateSigs' : Vector.t ADTSig m) *)
+(*              (DelegateReps' : Vector.t Type m) *)
+(*              (Delegatees := Build_NamedDelegatees DelegateSigs' DelegateReps') *)
+(*              (DelegateIDs := m) *)
+(*              (DelegateSigs := fun idx => *)
+(*                                 delegateeSig (Vector.nth Delegatees idx)) *)
+(*              (DelegateReps := fun idx => *)
+(*                                 delegateeRep (Vector.nth Delegatees idx)) *)
+(*              (rep : (Fin.t DelegateIDs -> Type) -> Type) *)
+(*              (cConstructors : *)
+(*                 forall *)
+(*                   (DelegateReps : Fin.t DelegateIDs -> Type) *)
+(*                   (DelegateImpls : forall idx, *)
+(*                                      ComputationalADT.pcADT (DelegateSigs idx) (DelegateReps idx)), *)
+(*                   ilist *)
+(*                     (B := fun Sig : consSig => *)
+(*                        ComputationalADT.cConstructorType *)
+(*                          (rep DelegateReps) (consDom Sig)) consSigs) *)
+(*              (cMethods : *)
+(*                 forall *)
+(*                   (DelegateReps : Fin.t DelegateIDs -> Type) *)
+(*                   (DelegateImpls : forall idx, *)
+(*                                      ComputationalADT.pcADT (DelegateSigs idx) (DelegateReps idx)), *)
+(*                   ilist *)
+(*                     (B := fun Sig : methSig => *)
+(*                        ComputationalADT.cMethodType *)
+(*                          (rep DelegateReps) (methDom Sig) *)
+(*                          (methCod Sig)) methSigs) *)
+(*              (DelegateSpecs' : ilist (B := fun nadt => ADT (delegateeSig nadt)) Delegatees ) *)
+(*              (DelegateSpecs := ith DelegateSpecs') *)
+(*              (cAbsR : *)
+(*                 forall *)
+(*                   (DelegateReps : Fin.t DelegateIDs -> Type) *)
+(*                   (DelegateImpls : forall idx, *)
+(*                                      ComputationalADT.pcADT (DelegateSigs idx) (DelegateReps idx)) *)
+(*                   (ValidImpls *)
+(*                    : forall idx : Fin.t DelegateIDs, *)
+(*                        refineADT (DelegateSpecs idx) *)
+(*                                  (ComputationalADT.LiftcADT (existT _ _ (DelegateImpls idx)))), *)
+(*                   RepT -> rep DelegateReps -> Prop) *)
+(*              (cConstructorsRefinesSpec : forall *)
+(*                                            (DelegateReps : Fin.t DelegateIDs -> Type) *)
+(*                                            (DelegateImpls : forall idx, *)
+(*                                                               ComputationalADT.pcADT (DelegateSigs idx) (DelegateReps idx)) *)
+(*                                            (ValidImpls *)
+(*                                             : forall idx : Fin.t DelegateIDs, *)
+(*                                                 refineADT (DelegateSpecs idx) *)
+(*                                                           (ComputationalADT.LiftcADT (existT _ _ (DelegateImpls idx)))), *)
+(*                                            Iterate_Dep_Type_BoundedIndex *)
+(*                                              (fun idx => *)
+(*                                                 @refineConstructor *)
+(*                                                   (RepT) (rep DelegateReps) (cAbsR _ _ ValidImpls) *)
+(*                                                   (consDom (Vector.nth consSigs idx)) *)
+(*                                                   (getConsDef consDefs idx) *)
+(*                                                   (LiftcConstructor _ _ (ith (cConstructors DelegateReps DelegateImpls) idx)))) *)
+(*              (cMethodsRefinesSpec : forall *)
+(*                                       (DelegateReps : Fin.t DelegateIDs -> Type) *)
+(*                                       (DelegateImpls : forall idx, *)
+(*                                                          ComputationalADT.pcADT (DelegateSigs idx) (DelegateReps idx)) *)
+(*                                       (ValidImpls *)
+(*                                        : forall idx : Fin.t DelegateIDs, *)
+(*                                            refineADT (DelegateSpecs idx) *)
+(*                                                      (ComputationalADT.LiftcADT (existT _ _ (DelegateImpls idx)))), *)
+(*                                       Iterate_Dep_Type_BoundedIndex *)
+(*                                         (fun idx => *)
+(*                                            @refineMethod *)
+(*                                              RepT (rep DelegateReps) *)
+(*                                              (cAbsR _ _ ValidImpls) *)
+(*                                              (methDom (Vector.nth methSigs idx)) *)
+(*                                              (methCod (Vector.nth methSigs idx)) *)
+(*                                              (getMethDef methDefs idx) *)
+(*                                              (LiftcMethod (ith (cMethods DelegateReps DelegateImpls) idx)))) *)
+(*   : FullySharpenedUnderDelegates *)
+(*       (BuildADT consDefs methDefs) *)
+(*       {| *)
+(*         Sharpened_DelegateSigs := DelegateSigs; *)
+(*         Sharpened_Implementation := Notation_Friendly_BuildMostlySharpenedcADT _ rep *)
+(*                                                                                cConstructors cMethods; *)
+(*         Sharpened_DelegateSpecs := DelegateSpecs |}. *)
+(*       refine (Notation_Friendly_FullySharpened_BuildMostlySharpenedcADT consDefs *)
+(*                                                                       methDefs _ rep cConstructors cMethods DelegateSpecs cAbsR *)
+(*                                                                       cConstructorsRefinesSpec cMethodsRefinesSpec). *)
+(*   Defined. *)
 
 End BuildADTRefinements.
 
-Arguments Notation_Friendly_BuildMostlySharpenedcADT _ _ _ _ _ _ _ _ _ _ _  / .
+(* Arguments Notation_Friendly_BuildMostlySharpenedcADT _ _ _ _ _ _ _ _ _ _ _  / . *)
 
-Ltac extract_delegate_free_impl :=
-  cbv beta; simpl;
-    match goal with
-        |- forall idx : Fin.t 0,
-             refineADT
-               (ith inil idx)
-               (ComputationalADT.LiftcADT
-                  (existT
-                     (ComputationalADT.pcADT
-                        (delegateeSig _))
-                     (?DelegateReps idx) (?DelegateSpecs idx))) =>
-        unify DelegateReps (fun idx : Fin.t 0 => False);
-          let P' := match type of DelegateSpecs with
-                    | forall idx, @?P' idx => P'
-                    end in
-          unify DelegateSpecs (fun idx : Fin.t 0 => Fin.case0 P' idx);
-            apply Fin.case0
-          end.
+(* Ltac extract_delegate_free_impl := *)
+(*   cbv beta; simpl; *)
+(*     match goal with *)
+(*         |- forall idx : Fin.t 0, *)
+(*              refineADT *)
+(*                (ith inil idx) *)
+(*                (ComputationalADT.LiftcADT *)
+(*                   (existT *)
+(*                      (ComputationalADT.pcADT *)
+(*                         (delegateeSig _)) *)
+(*                      (?DelegateReps idx) (?DelegateSpecs idx))) => *)
+(*         unify DelegateReps (fun idx : Fin.t 0 => False); *)
+(*           let P' := match type of DelegateSpecs with *)
+(*                     | forall idx, @?P' idx => P' *)
+(*                     end in *)
+(*           unify DelegateSpecs (fun idx : Fin.t 0 => Fin.case0 P' idx); *)
+(*             apply Fin.case0 *)
+(*           end. *)
 
-Tactic Notation "extract" "delegate-free" "implementation" :=
-  extract_delegate_free_impl.
+(* Tactic Notation "extract" "delegate-free" "implementation" := *)
+(*   extract_delegate_free_impl. *)
 
 (* A tactic for finishing a derivation. Probably needs a better name.*)
-Tactic Notation "finish" "sharpening" constr(delegatees):=
-  eexists; [ eapply reflexivityT
-           | constructor 1 with (Sharpened_DelegateSpecs := delegatees); intros;
-             split; simpl;
-             match goal with
-                 [|- forall idx : BoundedString, _] =>
-                 let idx := fresh in
-                 intro idx; pattern idx;
-                 eapply Iterate_Ensemble_BoundedIndex_equiv;
-                 unfold Iterate_Ensemble_BoundedIndex; simpl;
-                 intuition;
-                 repeat
-                   (try simplify with monad laws;
-                    first [constructor
-                          | match goal with
-                                |- context[if ?b then _ else _] =>
-                                destruct b
-                            end
-                          ])
-             end ].
+(* Tactic Notation "finish" "sharpening" constr(delegatees):= *)
+(*   eexists; [ eapply reflexivityT *)
+(*            | constructor 1 with (Sharpened_DelegateSpecs := delegatees); intros; *)
+(*              split; simpl; *)
+(*              match goal with *)
+(*                  [|- forall idx : BoundedString, _] => *)
+(*                  let idx := fresh in *)
+(*                  intro idx; pattern idx; *)
+(*                  eapply Iterate_Ensemble_BoundedIndex_equiv; *)
+(*                  unfold Iterate_Ensemble_BoundedIndex; simpl; *)
+(*                  intuition; *)
+(*                  repeat *)
+(*                    (try simplify with monad laws; *)
+(*                     first [constructor *)
+(*                           | match goal with *)
+(*                                 |- context[if ?b then _ else _] => *)
+(*                                 destruct b *)
+(*                             end *)
+(*                           ]) *)
+(*              end ]. *)
 
 Tactic Notation "finish" "honing" :=
   repeat match goal with
@@ -818,111 +818,111 @@ Ltac ilist_of_evar_dep n C D B As k :=
                                              ltac:(fun Bs' => k (fun (c : C) (d : D c) => icons (a := Vector.hd As) (b c d) (Bs' c d))))
   end.
 
-Ltac FullySharpenEachMethod DelegateSigs DelegateReps delegateSpecs :=
-    let Delegatees := constr:(Build_NamedDelegatees DelegateSigs DelegateReps) in
-    let DelegateSpecs := constr:(ith delegateSpecs) in
-    let NumDelegates := match type of DelegateSigs with
-                        | Vector.t _ ?n => n
-                        end in
-    match goal with
-      |- FullySharpenedUnderDelegates (@BuildADT ?Rep ?n ?n' ?consSigs ?methSigs ?consDefs ?methDefs) _ =>
-      ilist_of_evar_dep n
-        (Fin.t NumDelegates -> Type)
-        (fun D =>
-           forall idx,
-             ComputationalADT.pcADT (delegateeSig (Vector.nth Delegatees idx)) (D idx))
-        (fun Sig => ComputationalADT.cConstructorType Rep (consDom Sig))
-        consSigs
-        ltac:(fun cCons =>
-                ilist_of_evar_dep n'
-                                  (Fin.t NumDelegates -> Type)
-                                  (fun D =>
-                                     forall idx,
-             ComputationalADT.pcADT (delegateeSig (Vector.nth Delegatees idx)) (D idx))
-        (fun Sig => ComputationalADT.cMethodType Rep (methDom Sig) (methCod Sig))
-        methSigs
-        ltac:(fun cMeths =>
-                eapply (@Notation_Friendly_SharpenFully
-                          Rep NumDelegates n n'
-                          consSigs methSigs
-                          consDefs methDefs
-                          DelegateSigs DelegateReps
-                          (fun _ => Rep)
-                          cCons cMeths
-                          delegateSpecs
-                          (fun
-                         (DelegateReps'' : Fin.t NumDelegates -> Type)
-                         (DelegateImpls'' : forall idx,
-                             ComputationalADT.pcADT (delegateeSig (Vector.nth Delegatees idx)) (DelegateReps'' idx))
-                         (ValidImpls''
-                          : forall idx : Fin.t NumDelegates,
-                             refineADT (DelegateSpecs idx)
-                                       (ComputationalADT.LiftcADT (existT _ _ (DelegateImpls'' idx))))
-                            => @eq _)
-             )))
-    end; try (simpl; repeat split; intros; subst).
+(* Ltac FullySharpenEachMethod DelegateSigs DelegateReps delegateSpecs := *)
+(*     let Delegatees := constr:(Build_NamedDelegatees DelegateSigs DelegateReps) in *)
+(*     let DelegateSpecs := constr:(ith delegateSpecs) in *)
+(*     let NumDelegates := match type of DelegateSigs with *)
+(*                         | Vector.t _ ?n => n *)
+(*                         end in *)
+(*     match goal with *)
+(*       |- FullySharpenedUnderDelegates (@BuildADT ?Rep ?n ?n' ?consSigs ?methSigs ?consDefs ?methDefs) _ => *)
+(*       ilist_of_evar_dep n *)
+(*         (Fin.t NumDelegates -> Type) *)
+(*         (fun D => *)
+(*            forall idx, *)
+(*              ComputationalADT.pcADT (delegateeSig (Vector.nth Delegatees idx)) (D idx)) *)
+(*         (fun Sig => ComputationalADT.cConstructorType Rep (consDom Sig)) *)
+(*         consSigs *)
+(*         ltac:(fun cCons => *)
+(*                 ilist_of_evar_dep n' *)
+(*                                   (Fin.t NumDelegates -> Type) *)
+(*                                   (fun D => *)
+(*                                      forall idx, *)
+(*              ComputationalADT.pcADT (delegateeSig (Vector.nth Delegatees idx)) (D idx)) *)
+(*         (fun Sig => ComputationalADT.cMethodType Rep (methDom Sig) (methCod Sig)) *)
+(*         methSigs *)
+(*         ltac:(fun cMeths => *)
+(*                 eapply (@Notation_Friendly_SharpenFully *)
+(*                           Rep NumDelegates n n' *)
+(*                           consSigs methSigs *)
+(*                           consDefs methDefs *)
+(*                           DelegateSigs DelegateReps *)
+(*                           (fun _ => Rep) *)
+(*                           cCons cMeths *)
+(*                           delegateSpecs *)
+(*                           (fun *)
+(*                          (DelegateReps'' : Fin.t NumDelegates -> Type) *)
+(*                          (DelegateImpls'' : forall idx, *)
+(*                              ComputationalADT.pcADT (delegateeSig (Vector.nth Delegatees idx)) (DelegateReps'' idx)) *)
+(*                          (ValidImpls'' *)
+(*                           : forall idx : Fin.t NumDelegates, *)
+(*                              refineADT (DelegateSpecs idx) *)
+(*                                        (ComputationalADT.LiftcADT (existT _ _ (DelegateImpls'' idx)))) *)
+(*                             => @eq _) *)
+(*              ))) *)
+(*     end; try (simpl; repeat split; intros; subst). *)
 
-Ltac Implement_If_Then_Else :=
-  match goal with
-    | |- refine (If_Then_Else ?i (ret ?t) (ret ?e)) _ =>
-      apply (refine_If_Then_Else_ret i t e)
+(* Ltac Implement_If_Then_Else := *)
+(*   match goal with *)
+(*     | |- refine (If_Then_Else ?i (ret ?t) (ret ?e)) _ => *)
+(*       apply (refine_If_Then_Else_ret i t e) *)
 
-    | |- refine (Bind (If ?i Then ?t Else ?e) ?k) _ =>
-      etransitivity;
-        [ apply (refine_If_Then_Else_Bind i t e k)
-        | etransitivity;
-          [ apply refine_If_Then_Else;
-            [
-              | ]
-          | eapply refine_If_Then_Else_ret
-          ]
-        ]
-  end.
+(*     | |- refine (Bind (If ?i Then ?t Else ?e) ?k) _ => *)
+(*       etransitivity; *)
+(*         [ apply (refine_If_Then_Else_Bind i t e k) *)
+(*         | etransitivity; *)
+(*           [ apply refine_If_Then_Else; *)
+(*             [ *)
+(*               | ] *)
+(*           | eapply refine_If_Then_Else_ret *)
+(*           ] *)
+(*         ] *)
+(*   end. *)
 
-Ltac Implement_If_Opt_Then_Else :=
-  match goal with
-    | |- refine (Ifopt ?i as a Then (ret (@?t a)) Else (ret ?e)) _ =>
-      apply (refine_If_Opt_Then_Else_ret i t e)
+(* Ltac Implement_If_Opt_Then_Else := *)
+(*   match goal with *)
+(*     | |- refine (Ifopt ?i as a Then (ret (@?t a)) Else (ret ?e)) _ => *)
+(*       apply (refine_If_Opt_Then_Else_ret i t e) *)
 
-    | |- refine (Bind (Ifopt ?i as a Then (@?t a) Else ?e) ?k) _ =>
-      etransitivity;
-        [ apply (refine_If_Opt_Then_Else_Bind i t e k)
-        | etransitivity;
-          [ apply refine_If_Opt_Then_Else;
-            [ unfold pointwise_relation; intros
-              | ]
-          | eapply refine_If_Opt_Then_Else_ret
-          ]
-        ]
-  end.
+(*     | |- refine (Bind (Ifopt ?i as a Then (@?t a) Else ?e) ?k) _ => *)
+(*       etransitivity; *)
+(*         [ apply (refine_If_Opt_Then_Else_Bind i t e k) *)
+(*         | etransitivity; *)
+(*           [ apply refine_If_Opt_Then_Else; *)
+(*             [ unfold pointwise_relation; intros *)
+(*               | ] *)
+(*           | eapply refine_If_Opt_Then_Else_ret *)
+(*           ] *)
+(*         ] *)
+(*   end. *)
 
-Ltac finish_SharpeningADT_WithoutDelegation :=
-  eapply FullySharpened_Finish;
-  [ FullySharpenEachMethod
-      (@Vector.nil ADTSig)
-      (@Vector.nil Type)
-      (ilist.inil (B := fun nadt => ADT (delegateeSig nadt)));
-    try simplify with monad laws; simpl; try refine pick eq; try simplify with monad laws;
-    try first [ simpl];
-    (* Guard setoid rewriting with [refine_if_If] to only occur when there's *)
-(*     actually an [if] statement in the goal.  This prevents [setoid_rewrite] from *)
-(*     uselessly descending into folded definitions. *)
-    repeat lazymatch goal with
-             | [ |- context [ if _ then _ else _ ] ] =>
-               setoid_rewrite refine_if_If at 1
-           end;
-    repeat first [
-             higher_order_reflexivity
-           | simplify with monad laws
-           | Implement_If_Then_Else
-           | Implement_If_Opt_Then_Else ]
-  | extract_delegate_free_impl
-  | simpl; higher_order_reflexivityT ].
+(* Ltac finish_SharpeningADT_WithoutDelegation := *)
+(*   eapply FullySharpened_Finish; *)
+(*   [ FullySharpenEachMethod *)
+(*       (@Vector.nil ADTSig) *)
+(*       (@Vector.nil Type) *)
+(*       (ilist.inil (B := fun nadt => ADT (delegateeSig nadt))); *)
+(*     try simplify with monad laws; simpl; try refine pick eq; try simplify with monad laws; *)
+(*     try first [ simpl]; *)
+(*     (* Guard setoid rewriting with [refine_if_If] to only occur when there's *) *)
+(* (*     actually an [if] statement in the goal.  This prevents [setoid_rewrite] from *) *)
+(* (*     uselessly descending into folded definitions. *) *)
+(*     repeat lazymatch goal with *)
+(*              | [ |- context [ if _ then _ else _ ] ] => *)
+(*                setoid_rewrite refine_if_If at 1 *)
+(*            end; *)
+(*     repeat first [ *)
+(*              higher_order_reflexivity *)
+(*            | simplify with monad laws *)
+(*            | Implement_If_Then_Else *)
+(*            | Implement_If_Opt_Then_Else ] *)
+(*   | extract_delegate_free_impl *)
+(*   | simpl; higher_order_reflexivityT ]. *)
 
-Lemma refineIfret {A} :
-  forall (cond : bool) (a a' : A),
-    refine (if cond then ret a else ret a')
-           (ret (if cond then a else a')).
-Proof.
-  destruct cond; reflexivity.
-Qed.
+(* Lemma refineIfret {A} : *)
+(*   forall (cond : bool) (a a' : A), *)
+(*     refine (if cond then ret a else ret a') *)
+(*            (ret (if cond then a else a')). *)
+(* Proof. *)
+(*   destruct cond; reflexivity. *)
+(* Qed. *)
